riscV/Asm.v
@@ -1018,61 +1018,66 @@ Definition exec_instr (f: function) (i: instruction) (rs: regset) (m: mem) : out
        match Mem.record_frame (Mem.push_stage m1) (Memory.mk_frame sz) with
        |None => Stuck
        |Some m2 =>
-        let sp := Vptr stk Ptrofs.zero in
-        match Mem.storev Mptr m2 (Val.offset_ptr sp ofs_link) rs#SP with
-        | None => Stuck
-        | Some m3 => Next (nextinstr (rs #X30 <- (rs SP) #SP <- sp #X31 <- Vundef)) m3
-        end
+          let sp := Vptr stk Ptrofs.zero in
+          (* store return address *)
+          match Mem.storev Mptr m2 (Val.offset_ptr sp ofs_ra) rs#RA with
+          | None => Stuck
+          | Some m3 =>
+              match Mem.storev Mptr m3 (Val.offset_ptr sp ofs_link) rs#SP with
+              | None => Stuck
+              | Some m4 => Next (nextinstr (rs #X30 <- (rs SP) #SP <- sp #X31 <- Vundef)) m4
+              end
+          end
        end
      |_ => Stuck
       end
     else Stuck
-      (* let (m1, stk) := Mem.alloc m 0 sz in *)
-      (* let sp := (Vptr stk Ptrofs.zero) in *)
-      (* match Mem.storev Mptr m1 (Val.offset_ptr sp pos) rs#SP with *)
-      (* | None => Stuck *)
-      (* | Some m2 => Next (nextinstr (rs #X30 <- (rs SP) #SP <- sp #X31 <- Vundef)) m2 *)
-      (* end *)
-  | Pfreeframe sz ofs_ra ofs_link =>
-    (* if zle 0 sz then *)
-    (*   match Mem.loadv Mptr m (Val.offset_ptr rs#SP pos) with *)
-    (*   | None => Stuck *)
-    (*   | Some sp => *)
-    (*     match rs#SP with *)
-    (*     | Vptr stk ofs => *)
-    (*       if check_topframe sz (Mem.astack (Mem.support m)) then *)
-    (*         if Val.eq sp (parent_sp_stree (Mem.stack (Mem.support m))) then *)
-    (*           if Val.eq (Vptr stk ofs) (top_sp_stree (Mem.stack (Mem.support m))) then *)
-    (*               match Mem.free m stk 0 fsz with *)
-    (*               | None => Stuck *)
-    (*               | Some m' => *)
-    (*                 match Mem.return_frame m' with *)
-    (*                 | None => Stuck *)
-    (*                 | Some m'' => *)
-    (*                   match Mem.pop_stage m'' with *)
-    (*                     | None => Stuck *)
-    (*                     | Some m''' => *)
-    (*                     Next (nextinstr (rs#RSP <- sp #RA <- ra)) m''' *)
-    (*                   end *)
-    (*                 end *)
-    (*               end else Stuck else Stuck else Stuck *)
-    (*           | _ => Stuck *)
-    (*           end *)
-    (*       end *)
-    (*   end else Stuck *)
+
+  | Pfreeframe sz ofs_ra ofs_link =>      
+      if zle 0 sz then
+        match Mem.loadv Mptr m (Val.offset_ptr rs#SP ofs_ra) with
+        | None => Stuck
+        | Some ra =>
+            match Mem.loadv Mptr m (Val.offset_ptr rs#SP ofs_link) with
+            | None => Stuck
+            | Some sp =>
+                match rs#SP with
+                | Vptr stk ofs =>
+                    (* the following checking may be used in the SSAsm proof *)
+                    (* if check_topframe sz (Mem.astack (Mem.support m)) then *)
+                    (*   if Val.eq sp (parent_sp_stree (Mem.stack (Mem.support m))) then *)
+                    (*     if Val.eq (Vptr stk ofs) (top_sp_stree (Mem.stack (Mem.support m))) then *)
+                    match Mem.free m stk 0 sz with
+                    | None => Stuck
+                    | Some m' =>
+                        match Mem.return_frame m' with
+                        | None => Stuck
+                        | Some m'' =>
+                            match Mem.pop_stage m'' with
+                            | None => Stuck
+                            | Some m''' =>
+                                Next (nextinstr (rs#SP <- sp #RA <- ra #X31 <- Vundef)) m'''
+                            end
+                        end                          
+                    end
+                | _ => Stuck
+                end
+            end
+        end
+      else Stuck
     
-      match Mem.loadv Mptr m (Val.offset_ptr rs#SP ofs_link) with
-      | None => Stuck
-      | Some v =>
-          match rs SP with
-          | Vptr stk ofs =>
-              match Mem.free m stk 0 sz with
-              | None => Stuck
-              | Some m' => Next (nextinstr (rs#SP <- v #X31 <- Vundef)) m'
-              end
-          | _ => Stuck
-          end
-      end
+      (* match Mem.loadv Mptr m (Val.offset_ptr rs#SP ofs_link) with *)
+      (* | None => Stuck *)
+      (* | Some v => *)
+      (*     match rs SP with *)
+      (*     | Vptr stk ofs => *)
+      (*         match Mem.free m stk 0 sz with *)
+      (*         | None => Stuck *)
+      (*         | Some m' => Next (nextinstr (rs#SP <- v #X31 <- Vundef)) m' *)
+      (*         end *)
+      (*     | _ => Stuck *)
+      (*     end *)
+      (* end *)
   | Plabel lbl =>
       Next (nextinstr rs) m
   | Ploadsymbol rd s ofs =>
