riscV/Asmgenproof.v
@@ -364,7 +364,7 @@ Qed.
 Remark make_epilogue_label:
   forall f k, tail_nolabel k (make_epilogue f k).
 Proof.
-  unfold make_epilogue; intros. eapply tail_nolabel_trans. apply loadind_ptr_label. TailNoLabel.
+  unfold make_epilogue; intros. (* eapply tail_nolabel_trans. apply loadind_ptr_label. *) TailNoLabel.
 Qed.
 
 Lemma transl_instr_label:
